SystemFD/Metatheory/Cannonicity.lean
@@ -6,6 +6,8 @@ import SystemFD.Metatheory.FrameWf
 import SystemFD.Metatheory.Inversion
 import SystemFD.Reduction
 
+set_option maxHeartbeats 500000
+
 inductive Val : Ctx Term -> Term -> Prop where
 | app : t.neutral_form = .some (n, ts)
       -> (Γ.is_stable_red n)
@@ -58,7 +60,7 @@ case _ => cases ηJ; case _ fJ =>
 theorem cannonical_ctor_var :
   Γ ⊢ #h : T ->
   Γ ⊢ T : ★ ->
-  ValidCtor Γ T ->
+  ValidCtorType Γ T ->
   Γ.is_stable_red h ->
   Γ.is_ctor h := by
 intros tJ tstar vctor n_stable;
@@ -133,186 +135,50 @@ cases tJ; case _ wf h1 =>
     injection h1 with h1; cases h1;
     simp; rw [fh]; unfold Frame.is_insttype; simp;
 
-
--- @[simp]
--- abbrev ValidCtorSubtInvType : (v : JudgmentVariant) -> Ctx Term -> JudgmentArgs v -> Prop
--- | .prf => λ Δ => λ (A, τ) => ∀ Γ σ,
---     (∀ n y, σ n = .re y -> (Γ d@ n).apply σ = Δ d@ y) ->
---     (∀ n, Γ.is_stable n -> ∃ y, σ n = .re y) ->
---     ValidCtor Δ ([σ]A) ->
---     Δ ⊢ A : τ ->
---     (★ = τ) ->
---     ValidCtor Γ A
-
--- | .wf  => λ _ => λ () => true
-
--- theorem valid_ctor_subst_inv :
---   Judgment v Γ idx ->
---   ValidCtorSubtInvType v Γ idx
--- := by
--- intro j; induction j <;> simp at *;
--- all_goals (intro Γ σ f1 f2 vctor tJ)
--- all_goals try (intro e; subst e)
--- any_goals try (solve | cases tJ; case _ h _ => cases h)
--- any_goals try (solve | cases tJ; case _ h => cases h)
--- case _ =>
---   sorry
--- case _ =>
---   sorry
--- case _ aJ bJ ih1 ih2 =>
---   have ih1' := ih1 Γ σ f1 f2; -- stuck here as we have no easy way to build ValidCtor Γ ([σ] A)
---   have ih2' := ih2 Γ σ
---   sorry
--- case _ => cases vctor; sorry -- bogus case
--- case _ => exfalso; apply valid_ctor_not_equality vctor
--- case _ =>
---   sorry
--- case _ =>
---   sorry
--- case _ =>
---   sorry
-
-theorem valid_head_variable_subst_inv test σtest :
-  (∀ n, test n -> ∃ y, σ n = .re y ∧ σtest y) ->
-  (z = [σ]A) ->
-  ValidHeadVariable z σtest ->
-  ValidHeadVariable A test
-:= by
-intros f1 eq j; induction j <;> simp at *;
-case _ w fnf =>
-  unfold ValidHeadVariable;
-  exists w;
-  sorry
-
-
-theorem valid_ctor_subst_inv :
-    (∀ n y, σ n = .re y -> (Γ d@ n).apply σ = Δ d@ y) ->
-    (∀ n, Γ.is_stable n -> ∃ y, σ n = .re y) ->
-    Γ ⊢ A : τ ->
-    (★ = τ) ->
-    ([σ] A = Z) ->
-    ValidCtor Δ Z ->
-    ValidCtor Γ A
-:= by
-intro f1 f2 tJ eq1 eq2 j; induction j <;> simp at *;
-case refl vhv =>
-  subst eq1;
-  cases vhv; case _ Rnf =>
-  cases Rnf; case _ Rnf test =>
-
-  sorry
-case arrow ih =>
-
-  sorry
-case all ih =>
-
-  sorry
-
-inductive ArrowLike  : (T : Term) -> Prop where
-  | arrowt : ArrowLike (A -t> B)
-  | allt : ArrowLike (∀[A] B)
-
-@[simp]
-abbrev CannonicalCtorHeadType (Γ : Ctx Term) : (v : JudgmentVariant) -> JudgmentArgs v -> Prop
-| .prf => λ (t, τ) => ∀ h ts,
+theorem cannonical_ctor_head :
        Val Γ t ->
        Γ ⊢ t : τ ->
        Γ ⊢ τ : ★ ->
        t.neutral_form = .some (h, ts) ->
-       ValidCtor Γ τ ->
-       Γ.is_ctor h
-| .wf => λ () => true
+       (ValidCtorType Γ τ -> Γ.is_ctor h) ∨ (ValidInstType Γ τ -> Γ.is_insttype h) := by
+intro vt tJ τJ tnf;
+have tshape := Term.neutral_form_law (Eq.symm tnf)
+rw[<-tshape] at tJ;
+have hJ := inversion_apply_spine tJ;
+cases hJ; case _ τ' hJ =>
+cases hJ; case _ spTy hJ =>
+cases vt;
+any_goals(solve | cases tnf)
+case app h_stable tnf' =>
+  rw[tnf] at tnf'; cases tnf';
+  cases hJ; case _ wf gt =>
+  have τ'J := ctx_get_var_spine_type wf (Eq.symm gt) spTy τJ
+  simp at h_stable;
+  generalize fh : Γ d@ h = f at *;
+  cases f;
+  any_goals (solve | cases gt)
+  all_goals (unfold Frame.is_stable_red at h_stable; simp at h_stable)
+  all_goals (unfold Frame.get_type at gt; simp at gt; cases gt)
+  case _ =>
+    have h := ctx_get_var_type wf fh;
+    have uniq := uniqueness_of_types h τ'J; cases uniq;
+  case _ =>
+    have h := ctx_get_datatype_kind wf fh;
+    have uniq := uniqueness_of_types h τ'J; cases uniq;
+  case _ =>
+    apply Or.inl; intro vctor;
+    simp; rw[fh]; unfold Frame.is_ctor; simp;
+  case _ =>
+    have h := ctx_get_opent_kind wf fh
+    have uniq := uniqueness_of_types h τ'J; cases uniq;
+  case _ =>
+    apply Or.inr; intro vctor;
+    simp; rw[fh]; unfold Frame.is_insttype; simp;
 
-theorem cannonical_ctor_head :
-  Judgment v Γ idx ->
-  CannonicalCtorHeadType Γ v idx
- := by
-intros j; induction j <;> simp at *
-all_goals (intro n sp tv tJ τJ)
-any_goals try (solve | cases tv; case _ h => cases h)
-any_goals try (solve | apply Exists.intro 0;
-                         intro h; cases h; case _ h => cases h)
-case _ n τ wf gt _ =>
-  intro e1 e2 vctor;
-  subst e1; subst e2;
-  cases tv; case _ n sp nst ntf =>
-  cases ntf;
-  apply cannonical_ctor_var;
-  assumption; assumption; assumption; assumption
 
-all_goals (intro fnf vctor)
-case appk fJ aJ ih _ => -- bogus case
-  have lem := classification_lemma fJ; simp at lem
-  cases lem;
-  case _ h =>
-    cases h; case _ h =>
-    have uniq := uniqueness_of_types h τJ; cases uniq
-  case _ h =>
-    cases h; case _ h =>
-    cases h; case _ h h1 =>
-    cases h1; case _ h => cases h
-
-case _ Γ f A B a B' fJ aJ eq' ih1 _ =>
-  cases tv; case _ n ts ns fanf =>
-  simp at fanf; rw[Option.bind_eq_some] at fanf;
-  cases fanf; case _ w fnf' =>
-  cases fnf'; case _ fnf' fanf' =>
-  rw[Option.bind_eq_some] at fnf;
-  cases fnf; case _ w fnf =>
-  cases fnf; case _ fnf tsh =>
-  cases tsh;
-  rw[fnf] at fnf'; cases fnf';
-  cases fanf';
-  have lem := classification_lemma fJ; simp at lem;
-  cases lem;
-  case _ h => cases h;
-  case _ h =>
-  cases h; case _ h =>
-  cases h; case _ arrJ =>
-  have arrK := invert_arr_kind arrJ; subst arrK;
-  have h1 : ValidCtor (.empty::Γ) B := by
-    apply valid_ctor_subst_inv _ _ _ _ (Eq.symm eq') vctor; apply ★;
-    case _ =>
-      intro n y σ; induction n <;> simp at *;
-      rw[σ]; rw[Frame.apply_compose]; simp -- f1
-    case _ =>
-      intro n st; induction n <;> simp at *;
-      unfold Frame.is_stable at st; unfold Frame.apply at st; simp at *;
-    case _ => rw[eq'] at τJ; cases arrJ; assumption -- well typed
-    case _ => rfl -- ★ = ★
-  have h2 :ValidCtor Γ (A -t> B)  := ValidCtor.arrow h1;
-  apply ih1 w.fst w.snd (Val.app fnf ns) fJ arrJ fnf h2;
-
-case appt Γ f A B a B' fJ aJ eq' ih1 _ =>
-  cases tv; case _ n ts ns fanf =>
-  simp at fanf; rw[Option.bind_eq_some] at fanf;
-  cases fanf; case _ w fnf' =>
-  cases fnf'; case _ fnf' fanf' =>
-  rw[Option.bind_eq_some] at fnf;
-  cases fnf; case _ w fnf =>
-  cases fnf; case _ fnf tsh =>
-  cases tsh;
-  rw[fnf] at fnf'; cases fnf';
-  cases fanf';
-  have lem := classification_lemma fJ; simp at lem;
-  cases lem;
-  case _ h => cases h;
-  case _ h =>
-  cases h; case _ h =>
-  cases h; case _ arrJ =>
-  have arrK := invert_all_kind arrJ; subst arrK;
-  have h1 : ValidCtor (.kind A::Γ) B := by
-    apply valid_ctor_subst_inv _ _ _ _ (Eq.symm eq') vctor; apply ★;
-    case _ =>
-      intro n y σ; induction n <;> simp at *;
-      rw[σ]; rw[Frame.apply_compose]; simp -- f1
-    case _ =>
-      intro n st; induction n <;> simp at *;
-      unfold Frame.is_stable at st; unfold Frame.apply at st; simp at *;
-    case _ => rw[eq'] at τJ; cases arrJ; assumption -- well typed
-    case _ => rfl -- ★ = ★
-  have h2 :ValidCtor Γ (∀[A] B)  := ValidCtor.all h1;
-  apply ih1 w.fst w.snd (Val.app fnf ns) fJ arrJ fnf h2;
+inductive ArrowLike  : (T : Term) -> Prop where
+  | arrowt : ArrowLike (A -t> B)
+  | allt : ArrowLike (∀[A] B)
 
 inductive LambdaLike : (T : Term) -> Prop where
   | lam : LambdaLike (`λ[A] B)
@@ -325,7 +191,7 @@ abbrev CannonicalLambdaType (Γ : Ctx Term) : (v : JudgmentVariant) -> JudgmentA
        Γ ⊢ t : τ ->
        Γ ⊢ τ : ★ ->
        ArrowLike τ ->
-       ((LambdaLike t) ∨ (ValidHeadVariable t Γ.is_ctor ∨ ValidHeadVariable t Γ.is_insttype))
+       (LambdaLike t ∨ ValidHeadVariable t Γ.is_ctor ∨ ValidHeadVariable t Γ.is_insttype)
 | .wf => λ () => true
 
 theorem cannonical_lambda :
