SystemFD/Metatheory/Inversion.lean
@@ -6,12 +6,39 @@ import SystemFD.Metatheory.Uniqueness
 import SystemFD.Metatheory.FrameWf
 import SystemFD.Metatheory.Classification
 
+set_option maxHeartbeats 500000
+
+theorem invert_eq_kind : Γ ⊢ (A ~ B) : w -> w = ★ := by
+intros eqJ; cases eqJ; simp_all;
+
+theorem invert_arr_kind : Γ ⊢ (A -t> B) : w -> w = ★ := by
+intros eqJ; cases eqJ; simp_all;
+
+theorem invert_arrk_kind : Γ ⊢ (A -k> B) : w -> w = .kind := by
+intros eqJ; cases eqJ; simp_all;
+
+theorem invert_all_kind : (Γ ⊢ ∀[ A ] B : w) -> w = ★ := by
+intros eqJ; cases eqJ; simp_all;
+
+theorem lamt_typing_unique : Γ ⊢ Λ[A]b : t -> ∃ B', t = ∀[A] B' := by
+intros tJ; cases tJ; simp_all;
+
+theorem lam_typing_unique : Γ ⊢ `λ[A]b : t -> ∃ B', (t = (A -t> B')) := by
+intros tJ; cases tJ; simp_all;
+
+theorem refl_typing_unique : Γ ⊢ refl! A : t -> (t = (A ~ A)) := by
+intros tJ; cases tJ; simp_all;
+
+
 theorem inversion_apply_spine :
   Γ ⊢ t.apply_spine sp : A ->
   ∃ B, SpineType B A ∧ Γ ⊢ t : B
 := by
 intro j; induction sp generalizing Γ t A <;> simp at *
-case _ => exists A; apply And.intro SpineType.refl j
+case _ =>
+  exists A; apply And.intro;
+    apply SpineType.refl;
+  assumption
 case _ hd tl ih =>
   cases hd; case _ v a =>
   cases v <;> simp at *
@@ -20,24 +47,60 @@ case _ hd tl ih =>
     cases ih; case _ B ih =>
     cases ih; case _ h1 h2 =>
     cases h2; case _ C D j1 j2 j3 =>
-      subst j3; apply Exists.intro (C -t> D)
-      apply And.intro; apply SpineType.arrow; assumption; assumption;
+      have lem := classification_lemma j1; simp at lem;
+      cases lem;
+      case _ h =>
+        have uniq := invert_arr_kind h; cases uniq;
+      case _ h =>
+      cases h; case _ h =>
+        cases h; case _ h =>
+        have uniq := invert_arr_kind h; cases uniq;
+        subst j3; apply Exists.intro (C -t> D)
+        apply And.intro;
+          apply SpineType.arrow;
+          apply j2;
+          assumption;
+          assumption;
+        assumption
   case _ =>
     replace ih := ih j
     cases ih; case _ B ih =>
     cases ih; case _ h1 h2 =>
     cases h2; case _ C D j1 j2 j3 =>
-      subst j3; apply Exists.intro (∀[C] D)
-      apply And.intro; apply SpineType.all j2 h1
-      apply j1
+      have lem := classification_lemma j1; simp at lem;
+      cases lem;
+      case _ h =>
+        have uniq := invert_all_kind h; cases h
+      case _ h =>
+        cases h; case _ h =>
+        cases h; case _ h =>
+        have uniq := invert_all_kind h; cases uniq;
+        subst j3; apply Exists.intro (∀[C] D)
+        apply And.intro;
+          apply SpineType.all;
+          apply j2;
+          assumption;
+          apply h1;
+        apply j1
+
   case _ =>
     replace ih := ih j
     cases ih; case _ B ih =>
     cases ih; case _ j1 j2 =>
     cases j2; case _ C j2 j3 =>
-      apply Exists.intro (C -k> B)
-      apply And.intro; apply SpineType.arrowk j1
-      apply j3
+      have lem := classification_lemma j3; simp at lem;
+      cases lem;
+      case _ h =>
+        apply Exists.intro (C -k> B)
+        apply And.intro;
+        apply SpineType.arrowk;
+        assumption
+        apply j1;
+        assumption
+      case _ h =>
+        cases h; case _ h =>
+        cases h; case _ w h =>
+        have uniq := invert_arrk_kind h; cases h; cases w;
 
 theorem apply_spine_uniform :
   Γ ⊢ a : A ->
@@ -134,6 +197,37 @@ have lem1 := frame_wf_by_index x h1
 rw [h2] at lem1; cases lem1
 case _ j => apply j
 
+theorem ctx_get_var_type_star : ⊢ Γ -> Γ d@ x = .type t -> Γ ⊢ t : ★ := by
+intro h1 h2
+have lem1 := frame_wf_by_index x h1
+rw [h2] at lem1; cases lem1
+case _ j => apply j
+
+theorem ctx_get_var_ctor : ⊢ Γ -> Γ d@ x = .ctor t -> Γ ⊢ t : ★ := by
+intro h1 h2
+have lem1 := frame_wf_by_index x h1
+rw [h2] at lem1; cases lem1
+case _ => assumption
+
+theorem ctx_get_var_insttype : ⊢ Γ -> Γ d@ x = .insttype t -> Γ ⊢ t : ★ := by
+intro h1 h2
+have lem1 := frame_wf_by_index x h1
+rw [h2] at lem1; cases lem1
+case _ => assumption
+
+theorem ctx_get_var_openm : ⊢ Γ -> Γ d@ x = .openm t -> Γ ⊢ t : ★ := by
+intro h1 h2
+have lem1 := frame_wf_by_index x h1
+rw [h2] at lem1; cases lem1
+case _ => assumption
+
+theorem ctx_get_var_term : ⊢ Γ -> Γ d@ x = .term t t' -> Γ ⊢ t : ★ := by
+intro h1 h2
+have lem1 := frame_wf_by_index x h1
+rw [h2] at lem1; cases lem1
+case _ => assumption
+
+
 theorem ctx_get_var_no_eq_type :
   ⊢ Γ ->
   Γ.is_stable_red x ->
@@ -176,7 +270,7 @@ case _ j ih =>
     apply ih h2 h3
 
 theorem valid_ctor_not_equality :
-  ¬ (ValidCtor Γ (A ~ B))
+  ¬ (ValidCtorType Γ (A ~ B))
 := by
 intro h
 generalize Tdef : (A ~ B) = T at *
@@ -190,7 +284,7 @@ case _ => injection Tdef
 theorem spine_type_is_not_valid_ctor :
   T = (C ~ D) ->
   SpineType A T ->
-  ValidCtor Γ A ->
+  ValidCtorType Γ A ->
   False
 := by
 intro e h1 h2
@@ -312,23 +406,21 @@ case _ j1 j2 => subst h3; apply spine_type_is_not_valid_ctor rfl h5 j2
 case _ j => subst h3; apply spine_type_is_not_kind h5 h4 j
 case _ j1 j2 => subst h3; apply spine_type_is_not_valid_insttype rfl h5 j2
 
-theorem invert_eq_kind : Γ ⊢ (A ~ B) : w -> w = ★ := by
-intros eqJ; cases eqJ; simp_all;
-
-theorem invert_arr_kind : Γ ⊢ (A -t> B) : w -> w = ★ := by
-intros eqJ; cases eqJ; simp_all;
-
-theorem invert_all_kind : (Γ ⊢ ∀[ A ] B : w) -> w = ★ := by
-intros eqJ; cases eqJ; simp_all;
-
-theorem lamt_typing_unique : Γ ⊢ Λ[A]b : t -> ∃ B', t = ∀[A] B' := by
-intros tJ; cases tJ;
-case _ => simp_all;
-
-theorem lam_typing_unique : Γ ⊢ `λ[A]b : t -> ∃ B', (t = (A -t> B')) := by
-intros tJ; cases tJ;
-case _ => simp_all;
-
-theorem refl_typing_unique : Γ ⊢ refl! A : t -> (t = (A ~ A)) := by
-intros tJ; cases tJ;
-case _ => simp_all;
+theorem ctx_get_var_spine_type :
+  ⊢ Γ ->
+  (Γ d@ n).get_type = some τ' ->
+  SpineType τ' τ ->
+  Γ ⊢ τ : ★ ->
+  Γ ⊢ τ' : ★ := by
+intro wf gt spTy τJ;
+have spk := spine_type_is_not_kind spTy τJ
+unfold Frame.get_type at gt; split at gt;
+all_goals (cases gt)
+case _ f => have f' := ctx_get_var_type wf f; exfalso; apply spk f'
+case _ f => apply ctx_get_var_type_star wf f
+case _ f => have f' := ctx_get_datatype_kind wf f; exfalso; apply spk f'
+case _ f => apply ctx_get_var_ctor wf f
+case _ f => have f' := ctx_get_opent_kind wf f; exfalso; apply spk f'
+case _ f => apply ctx_get_var_openm wf f
+case _ f => apply ctx_get_var_insttype wf f
+case _ f => apply ctx_get_var_term wf f
